# A Model of Time-Dependent Random Noise

Following is a simple model of time-dependent random noise. While this model can be useful as a motivation for the `bench_diff` approach, the test benchmarks discussed previously provide independent validation of the benchmarking approach used in this library.

**Definitions and assumptions:**

1. Let **ln(x)** be the natural logarithm of **x**.
2. Let **L(f, t)** be the latency of function **f** at time **t**.
3. Let **λ1** be the baseline (ideal) latency of function **f1** in the absence of noise; respectively, **λ2** for **f2**.
4. Given a random variable **χ**, let **E(χ)** and **Stdev(χ)** be the expected value and standard deviation of **χ**, respectively.
5. Assume time-dependent noise is **ν(t) = α(t) * β(t)**, where:
   - **α(t)** > 0 is a smooth deterministic function of **t**, such that there are constants **A<sub>L</sub>**, **A<sub>U</sub>**, and **A<sub>D</sub>** for which **A<sub>L</sub> <= α(t) <= A<sub>U</sub>** and **|α'(t)| <= A<sub>D</sub>**, for all **t**.
   - **β(t)** is a random variable dependent on **t**, with a log-normal distribution, such that **E(ln(β(t))) = 0** and **Stdev(ln(β(t))) = σ**, where **σ** is a constant that does not depend on **t**.
6. Assume **L(f1, t) = λ1 * ν(t)** and **L(f2, t) = λ2 * ν(t)** for all **t**.

**Implications:**

1. When we measure **f1**'s latency at a time **t<sub>1</sub>**, getting **L(f1, t<sub>1</sub>)**, and right after we measure **f2**'s latency, the measurement for **f2** occurs at a time **t<sub>2</sub> = t<sub>1</sub> + Δt<sub>1</sub>**, where **Δt<sub>1</sub>** is <u>very close</u> to **L(f1, t<sub>1</sub>)**.

2. Substituting *assumption 5* into *assumption 6* for **f1** at time **t<sub>1</sub>** and **f2** at time **t<sub>2</sub> = t<sub>1</sub> + Δt<sub>1</sub>**:

   - **L(f1, t<sub>1</sub>) = λ1 * α(t<sub>1</sub>) * β(t<sub>1</sub>)**
   - **L(f2, t<sub>2</sub>) = λ2 * α(t<sub>1</sub> + Δt<sub>1</sub>) * β(t<sub>2</sub>)**

3. Applying natural logarithms on *implication 2*:

   - **ln(L(f1, t<sub>1</sub>)) = ln(λ1) + ln(α(t<sub>1</sub>)) + ln(β(t<sub>1</sub>))**
   - **ln(L(f2, t<sub>2</sub>)) = ln(λ2) + ln(α(t<sub>1</sub> + Δt<sub>1</sub>)) + ln(β(t<sub>2</sub>))** 

4. Based on the bound on **α'(t)** from *assumption 5*:

   - ln(α(t<sub>1</sub> + Δt<sub>1</sub>))  

     = ln(α(t<sub>1</sub>)) + Δt<sub>1</sub> * α'(t<sub>p</sub>)/α(t<sub>p</sub>)  **[**_for some t<sub>p</sub> between t<sub>1</sub> and Δt<sub>1</sub>_**]**  

     = ln(α(t<sub>1</sub>)) + Δt<sub>1</sub> * γ(t<sub>1</sub>)/α(t<sub>p</sub>)  **[**_where |γ(t<sub>1</sub>)| <= A<sub>D</sub>_**]**

   Based on the bounds for **α(t)** from *assumption 5*:
   - 1 / α(t<sub>p</sub>) - 1 / α(t<sub>1</sub>)  

     = -α'(t<sub>q</sub>) / α(t<sub>1</sub>)^2  **[**_for some t<sub>q</sub> between t<sub>1</sub> and t<sub>p</sub>_**]**  

     = δ<sub>0</sub>(t<sub>1</sub>) / α(t<sub>1</sub>)  **[**_where |δ<sub>0</sub>(t<sub>1</sub>)| <= A<sub>D</sub>/A<sub>L</sub>_**]**  

     Thus:  

     1 / α(t<sub>p</sub>)  

     = 1 / α(t<sub>1</sub>) + δ<sub>0</sub>(t<sub>1</sub>) / α(t<sub>1</sub>)  

     = (1 + δ<sub>0</sub>(t<sub>1</sub>)) / α(t<sub>1</sub>)  

     = δ(t<sub>1</sub>) / α(t<sub>1</sub>)  **[**_where 1 - A<sub>D</sub>/A<sub>L</sub> <= δ(t<sub>1</sub>) <= 1 + A<sub>D</sub>/A<sub>L</sub>_**]**

   Therefore, from the first equation in this implication group and the above equation:

   - ln(α(t<sub>1</sub> + Δt<sub>1</sub>))  

     = ln(α(t<sub>1</sub>)) + Δt<sub>1</sub> * γ(t<sub>1</sub>) * δ(t<sub>1</sub>) / α(t<sub>1</sub>)  

     = ln(α(t<sub>1</sub>)) + Δt<sub>1</sub> * ε<sub>1</sub>(t<sub>1</sub>) / α(t<sub>1</sub>)  **[**_where ε<sub>1</sub>(t<sub>1</sub>) = γ(t<sub>1</sub>) * δ(t<sub>1</sub>)  and  |ε<sub>1</sub>(t<sub>1</sub>)| <= A<sub>D</sub> * (1 +  A<sub>D</sub> / A<sub>L</sub>) =<sub>def</sub> ε<sub>1</sub><sup>U</sup>_**]**  
     
     Alternatively:  **[**_ε<sub>1</sub><sup>U</sup> = A<sub>D</sub> * (1 +  A<sub>D</sub> / A<sub>L</sub>)_**]**

5. Applying *implication 4* to *implication 3*:

   - ln(L(f1, t<sub>1</sub>)) = ln(λ1) + ln(α(t<sub>1</sub>)) + ln(β(t<sub>1</sub>))

   - ln(L(f2, t<sub>2</sub>))  

     = ln(λ2) + ln(α(t<sub>1</sub>)) + Δt<sub>1</sub> * ε<sub>1</sub>(t<sub>1</sub>)/α(t<sub>1</sub>) + ln(β(t<sub>2</sub>))   **[**_where |ε<sub>1</sub>(t<sub>1</sub>)| <= ε<sub>1</sub><sup>U</sup>_**]**  

     Using *implication 1* to replace the **Δt<sub>1</sub>** value in the in the second equation of *implication 5*:  

     = ln(L(f2, t<sub>2</sub>)) = ln(λ2) + ln(α(t<sub>1</sub>)) + L(f1, t<sub>1</sub>) * ε<sub>1</sub>(t<sub>1</sub>)/α(t<sub>1</sub>) + ln(β(t<sub>2</sub>))  

     Using *implication 1* to replace the **Δt<sub>1</sub>** value in the in the second equation of *implication 5*:

6. Using the first equation in *implication 2* and the formula for the expected value of a log-normal distribution:

   - E(L(f1, t<sub>1</sub>))  

     = λ1 * α(t<sub>1</sub>) * E(β(t<sub>1</sub>))  

     = λ1 * α(t<sub>1</sub>) * exp(σ<sup>2</sup>/2)

7. Taking expected values in *implication 5*:

   - E(ln(L(f1, t<sub>1</sub>))) = ln(λ1) + ln(α(t<sub>1</sub>)) + E(ln(β(t<sub>1</sub>)))
   - E(ln(L(f2, t<sub>2</sub>))) = ln(λ2) + ln(α(t<sub>1</sub>)) + E(ε<sub>1</sub>(t<sub>1</sub>) * L(f1, t<sub>1</sub>)) / α(t<sub>1</sub>) + E(ln(β(t<sub>2</sub>)))

8. Using the second item in *assumption 5*, *implication 7* simplifies to:

   - E(ln(L(f1, t<sub>1</sub>))) = ln(λ1) + ln(α(t<sub>1</sub>))
   - E(ln(L(f2, t<sub>2</sub>))) = ln(λ2) + ln(α(t<sub>1</sub>)) + E(ε<sub>1</sub>(t<sub>1</sub>) * L(f1, t<sub>1</sub>)) / α(t<sub>1</sub>)  

9.  By standard expected value inequalities:

   - |E(ε<sub>1</sub>(t<sub>1</sub>) * L(f1, t<sub>1</sub>))|  

     <= E(|ε<sub>1</sub>(t<sub>1</sub>)| * |L(f1, t<sub>1</sub>)|)  

     <= E(|ε<sub>1</sub>(t<sub>1</sub>)|) * E(|L(f1, t<sub>1</sub>)|)  

     = E(|ε<sub>1</sub>(t<sub>1</sub>)|) * E(L(f1, t<sub>1</sub>))  

     Using the  bound|ε<sub>1</sub>(t<sub>1</sub>)| <= ε<sub>1</sub><sup>U</sup> from *implicaition 4*:

     <= ε<sub>1</sub><sup>U</sup> * E(L(f1, t<sub>1</sub>))  

     By *implication 6*:

     = ε<sub>1</sub><sup>U</sup> * λ1 * α(t<sub>1</sub>) * exp(σ<sup>2</sup>/2)

10. Using *implication 9* and substituting *implication 7* into the second equation:

       - **E(ln(L(f1, t<sub>1</sub>))) = ln(λ1) + ln(α(t<sub>1</sub>))**
       - **E(ln(L(f2, t<sub>2</sub>)))  
         = ln(λ2) + ln(α(t<sub>1</sub>)) + α'(t<sub>1</sub>)/α(t<sub>1</sub>) * λ1 * α(t<sub>1</sub>) * exp(1/2 * σ^2) + E(ε<sub>1</sub>(t<sub>1</sub>))  
         = ln(λ2) + ln(α(t<sub>1</sub>)) + α'(t<sub>1</sub>) * λ1 * exp(1/2 * σ^2) + E(ε<sub>1</sub>(t<sub>1</sub>))**

11. Subtracting the second equation from the first in *implication 9* and using the linearity of **E()**:

    - **E(ln(L(f1, t<sub>1</sub>) - ln(L(f2, t<sub>2</sub>))))**  
      **= ln(λ1) - ln(λ2) - α'(t<sub>1</sub>) * λ1 * exp(1/2 * σ^2) - E(ε<sub>1</sub>(t<sub>1</sub>)) **  
      **= ln(λ1 / λ2) - α'(t<sub>1</sub>) * λ1 * exp(1/2 * σ^2) - E(ε<sub>1</sub>(t<sub>1</sub>))**

12. With `bench_diff`, measurements are done pairs, with one half of the pairs having **f1** followed by **f2** and the other half having **f2** followed by **f1**. The equation in *implication 10* above pertains to the first case. The analogous equation for the second case is:
    - **E(ln(L(f2, t<sub>2'</sub>) - ln(L(f1, t<sub>1'</sub>)))) = ln(λ2 / λ1) - α'(t<sub>2'</sub>) * λ2 * exp(1/2 * σ^2) - E(ε<sub>2</sub>(t<sub>2'</sub>))**
      or, equivalently: 
    - **E(ln(L(f1, t<sub>1'</sub>)) - ln(L(f2, t<sub>2'</sub>))) = ln(λ1 / λ2) + α'(t<sub>2'</sub>) * λ2 * exp(1/2 * σ^2) + E(ε<sub>2</sub>(t<sub>2'</sub>))**

13. Assuming the number of latency observations for each function is **n** and considering the two cases as described in *implication 11*, we can calculate the sample mean difference between the natural logarithms of the observed latencies:
    - **mean_diff_ln =**  
      **1/n * ∑<sub>i=1..n</sub> (ln(L(f1, t<sub>1<sub>i</sub></sub>) - ln(L(f2, t<sub>2<sub>i</sub></sub>)) **
      **= 1/n * (∑<sub>i:odd</sub> (ln(L(f1, t<sub>1<sub>i</sub></sub>) - ln(L(f2, t<sub>2<sub>i</sub></sub>)) + ∑<sub>i:even</sub> (ln(L(f1, t<sub>1<sub>i</sub></sub>) - ln(L(f2, t<sub>2<sub>i</sub></sub>)))**

14. Using the linearity of **E()** and calculating the definition of the sample mean **M(i, x<sub>i</sub>)** for a sample **x** with observations **x<sub>1</sub>, ..., x<sub>i</sub>, ..., x<sub>n</sub>**:
    - **∑<sub>i:odd</sub> x<sub>i</sub>**
    - **E(M(i, ln(L(f1, t<sub>1<sub>i</sub></sub>) - ln(L(f2, t<sub>2<sub>i</sub></sub>))))) = M(i, E(ln(L(f1, t<sub>1<sub>i</sub></sub>) - ln(L(f2, t<sub>2<sub>i</sub></sub>)))))**

15. Using *implication 13* and taking the sample mean **M()** of each side in *implication 10* and *implication 12* over all measured latencies, we get:

    - **E(M(i, ln(L(f1, t<sub>1<sub>i</sub></sub>) - ln(L(f2, t<sub>2<sub>i</sub></sub>)))) = ln(λ1 / λ2) - M(i, α'(t<sub>1<sub>i</sub></sub>)) * λ1 * exp(1/2 * σ^2) - M(i, E(ε<sub>1</sub>(t<sub>1<sub>i</sub></sub>))))**
    - **E(M(i, ln(L(f1, t<sub>1'<sub>i</sub></sub>) - ln(L(f2, t<sub>2'<sub>i</sub></sub>)))) = ln(λ1 / λ2) + M(i, α'(t<sub>2'<sub>i</sub></sub>)) * λ2 * exp(1/2 * σ^2) + M(i, E(ε<sub>2</sub>(t<sub>2'<sub>i</sub></sub>))))**

16. Both equations in *implication 14* show that the difference between the sample means of the natural logarithms of the observed latencies is an approximately unbiased estimator of **ln(λ1 / λ2)**. The bias is equal to the following equivalent values:

    - **- M(i, α'(t<sub>1<sub>i</sub></sub>)) * λ1 * exp(1/2 * σ^2) - M(i, E(ε<sub>1</sub>(t<sub>1<sub>i</sub></sub>)))**
    - **M(i, α'(t<sub>2'<sub>i</sub></sub>)) * λ2 * exp(1/2 * σ^2) + M(i, E(ε<sub>2</sub>(t<sub>2'<sub>i</sub></sub>)))**

17. Thus, assuming the rate of change of **α(t)** is sufficiently small for all **t** during the measurement process, the estimates of the ratio of latency medians produced by `bench_diff` should be sufficiently accurate.


# Limitations

This library works well for latencies at the microseconds or millisecodns order of magnitude, but not for latencies at the nanoseconds order of magnitude.